CertiGC/verif_forward2.v
@@ -22,7 +22,7 @@ Lemma body_forward_intr:
     (rsh sh : share)
     (gv : globals)
     (g : LGraph)
-    (h : heap)
+    (h : part_heap)
     (hp : val)
     (outlier : outlier_t)
     (from to : nat)
@@ -45,7 +45,7 @@ Lemma body_forward_intr:
          SEP (all_string_constants rsh gv; outlier_rep outlier;
               graph_rep g; heap_rep sh h hp)) (fn_body f_forward)
       (normal_ret_assert
-         ((EX (g' : LGraph) (h' : heap),
+         ((EX (g' : LGraph) (h' : part_heap),
             PROP ((g', h') =
                     forward_graph_and_heap from to (Z.to_nat depth)
                       (forward_p2forward_t (FwdPntIntr intr) g) g h)
@@ -457,7 +457,7 @@ Proof.
                    subst gg g'. apply lcv_outlier_compatible; assumption. }
                 forward_for_simple_bound
                   n'
-                    (EX i: Z, EX g3: LGraph, EX h3: heap,
+                    (EX i: Z, EX g3: LGraph, EX h3: part_heap,
                             PROP ((g3, h3) = forward_gh_loop forward_graph_and_heap
                                                from to (Z.to_nat (depth - 1))
                                                (sublist 0 i (vertex_pos_pairs gg ncv))
